

1) a)

1. Let l be likelihood

$$\log l = \sum_{i=1}^m \log \left(\frac{1}{2\pi n^{1/2}} e^{-\frac{1}{2}(\bar{x}_i - \bar{\mu})^T \Sigma^{-1}(\bar{x}_i - \bar{\mu})} \right)$$

where $\Sigma \Rightarrow$ Covariance Matrix, $n \Rightarrow$ Dimension of \bar{x}_i vector
 $\bar{\mu} \Rightarrow$ Mean vector

$$\Rightarrow \log l = -\sum_{i=1}^m \left(\log 2\pi^{n/2} + \frac{1}{2} \log |\Sigma| + \frac{1}{2} (\bar{x}_i - \bar{\mu})^T \Sigma^{-1} (\bar{x}_i - \bar{\mu}) \right)$$

To get maximize likelihood (log likelihood),

$$\frac{\partial \log l}{\partial \bar{\mu}} = 0, \quad \frac{\partial \log l}{\partial \Sigma} = 0$$

$$+ \frac{\partial \log l}{\partial \bar{\mu}} = -\sum_{i=1}^m \left(\frac{1}{2|\Sigma|} \frac{\partial |\Sigma|}{\partial \bar{\mu}} + \frac{1}{2} \frac{\partial}{\partial \bar{\mu}} \left((\bar{x}_i - \bar{\mu})^T \Sigma^{-1} (\bar{x}_i - \bar{\mu}) \right) \right)$$

$$\Rightarrow \frac{\partial \log l}{\partial \bar{\mu}} = -\sum_{i=1}^m \left(0 + \frac{1}{2} (-2 \Sigma^{-1} (\bar{x}_i - \bar{\mu})) \right)$$

As, $\frac{\partial (t^T A t)}{\partial t} = (A + A^T) t$, Here Σ^{-1} is A where Σ is symmetric, hence derivative is $2 \Sigma^{-1} (\bar{x}_i - \bar{\mu})$. Also we have $(\bar{x}_i - \bar{\mu})$ so extra minus comes

$$\bar{\mu} = \frac{1}{m} \sum_{i=1}^m \bar{x}_i$$

\Rightarrow

$$\left(\begin{pmatrix} 1 \\ 1 \\ \vdots \\ 1 \end{pmatrix} \right)^T \left(\begin{pmatrix} \bar{x}_1 \\ \bar{x}_2 \\ \vdots \\ \bar{x}_m \end{pmatrix} \right) = \left(\begin{pmatrix} \bar{x}_1 \\ \bar{x}_2 \\ \vdots \\ \bar{x}_m \end{pmatrix} \right)^T \left(\begin{pmatrix} 1 \\ 1 \\ \vdots \\ 1 \end{pmatrix} \right)$$

$$\frac{\partial \log l}{\partial \Sigma} = - \sum_{i=1}^m \left(\frac{1}{2} \Sigma^{-1} + \frac{1}{2} \frac{\partial}{\partial \Sigma} ((\bar{x}_i - \bar{\mu})^T \Sigma^{-1} (\bar{x}_i - \bar{\mu})) \right)$$

$$(A) \frac{\partial \log |A|}{\partial A} = (A^{-1})^T$$

$$\Rightarrow \frac{\partial \log l}{\partial \Sigma^{-1}} = - \sum_{i=1}^m \frac{1}{2} \Sigma + \frac{1}{2} (\bar{x}_i - \bar{\mu})(\bar{x}_i - \bar{\mu})^T$$

($\frac{\partial}{\partial \Sigma^{-1}}$ operator is used, as we have Σ^{-1} in RHS)

$$(AS \quad (\bar{x}_i - \bar{\mu})^T \Sigma^{-1} (\bar{x}_i - \bar{\mu}) = \text{Tr}((\bar{x}_i - \bar{\mu})(\bar{x}_i - \bar{\mu})^T \Sigma^{-1})) \quad (\text{Tr}(BCA) = \text{Tr}(ABC))$$

$$\Sigma = \frac{1}{m} \sum_{i=1}^m (\bar{x}_i - \bar{\mu})(\bar{x}_i - \bar{\mu})^T$$

$$\text{Tr}(X^T A X) = X^T A X \text{ as } X^T A X \text{ is Scalar}$$

(b)
MAP

* Lets assume Normal prior for $(\bar{\mu}_{MAP})_{\text{prior}} \sim N(\bar{\mu}, \Sigma)$ (Multivariate)

* Lets take $\bar{\mu} = \bar{\mu}_{MLE}$, $\Sigma = \Sigma_{MLE} \Rightarrow (\bar{\mu}_{MAP})_{\text{prior}} \sim N(\bar{\mu}_{MLE}, \Sigma_{MLE})$

* Let $\bar{\mu}_{MLE} = \bar{\mu}_0$, $\Sigma_{MLE} = \Sigma_0$

$$\bullet \text{ argmax } \left(\frac{1}{\sigma} \frac{f(\theta)}{x_1, x_2, \dots, x_n} \right) = \text{argmax} \left(\frac{1}{\sigma} (x_1, x_2, \dots, x_n) \cdot f(\theta) \right)$$

\Rightarrow

$$\text{argmax} \left(N\left(\frac{\bar{\mu}}{\text{Data}}\right) \right) = \text{argmax} \left(N\left(\frac{\text{Data}}{\bar{\mu}}\right) \cdot N(\bar{\mu}) \right)$$

27
135

$$\Rightarrow \log(\text{argmax}_{\bar{\mu}} \left(N(\bar{\mu} | \text{Data}) \right)) = \sum_{i=1}^m \log \left(\frac{1}{2\pi^{D/2} |\Sigma|^{1/2}} e^{-\frac{1}{2} (\bar{x}_i - \bar{\mu})^T \Sigma^{-1} (\bar{x}_i - \bar{\mu})} \right) + \log \left(\frac{1}{2\pi^{D/2} |\Sigma_0|^{1/2}} e^{-\frac{1}{2} (\bar{\mu} - \bar{\mu}_0)^T \Sigma_0^{-1} (\bar{\mu} - \bar{\mu}_0)} \right)$$

$$\Rightarrow \frac{\partial \log(\text{argmax}_{\bar{\mu}} \left(N(\bar{\mu} | \text{Data}) \right))}{\partial \bar{\mu}} = \left(\sum_{i=1}^m \left(0 + \frac{1}{2|\Sigma|} \frac{\partial |\Sigma|}{\partial \bar{\mu}} + \frac{1}{2} (-2 \Sigma^{-1} (\bar{x}_i - \bar{\mu})) \right) + \left(0 + \frac{1}{|\Sigma_0|} \frac{\partial |\Sigma_0|}{\partial \bar{\mu}} + \frac{1}{2} (-2 \Sigma_0^{-1} (\bar{\mu} - \bar{\mu}_0)) \right) \right)$$

$$\Rightarrow \frac{\partial \log(\text{argmax}_{\bar{\mu}} \left(N(\bar{\mu} | \text{Data}) \right))}{\partial \bar{\mu}} = - \sum_{i=1}^m \Sigma^{-1} (\bar{x}_i - \bar{\mu}) + \Sigma_0^{-1} (\bar{\mu} - \bar{\mu}_0)$$

$$\Rightarrow \bar{\mu}_{\text{MAP}} = \left(\Sigma_0^{-1} + m \Sigma^{-1} \right) \left(\Sigma_0^{-1} \bar{\mu}_0 + \sum_{i=1}^m (\Sigma^{-1} \bar{x}_i) \right)$$

Q2)

$$E\left(\frac{1}{m} \sum_{i=1}^m (\bar{x}_i - \bar{\mu})(\bar{x}_i - \bar{\mu})^T\right) = \frac{1}{m} E\left(\sum_{i=1}^m (\bar{x}_i \bar{x}_i^T - \bar{\mu} \bar{x}_i^T - \bar{x}_i \bar{\mu}^T + \bar{\mu} \bar{\mu}^T)\right)$$

$$\Rightarrow \frac{1}{m} E\left(\sum_{i=1}^m (\bar{x}_i \bar{x}_i^T - \bar{\mu} \bar{\mu}^T)\right)$$

$$\Rightarrow \frac{1}{m} E\left(\sum_{i=1}^m (\bar{x}_i \bar{x}_i^T) - \frac{1}{m} \sum_{i=1}^m (\bar{\mu} \bar{x}_i^T + \bar{x}_i \bar{\mu}^T)\right)$$

$$\Rightarrow \frac{1}{m} E\left(\sum_{i=1}^m (\bar{x}_i \bar{x}_i^T) - \frac{1}{m} \sum_{i=1}^m (\bar{\mu} \bar{x}_i^T + \bar{x}_i \bar{\mu}^T)\right)$$

$$\Rightarrow \frac{1}{m} \left(m \mu_{xx}^T - \frac{1}{m} (m \mu_{xx}^T + m(m-1) \mu_{x0} \mu_{x0}^T) \right)$$

$$\Rightarrow \left(\frac{m-1}{m} \right) (\mu_{xx}^T - \mu_{x0} \mu_{x0}^T)$$

$$\Rightarrow E(\hat{\Sigma}) = \left(\frac{m-1}{m} \right) \sigma_{xx}^T$$

For $\hat{\Sigma}$ to be unbiased estimator, $\hat{\Sigma}$ has to be unbiased

$$\hat{\Sigma} = \frac{1}{m} \sum_{i=1}^m (\bar{x}_i - \bar{\mu})(\bar{x}_i - \bar{\mu})^T$$

$$\hat{\Sigma} = \frac{1}{m} \sum_{i=1}^m (\bar{x}_i \bar{x}_i^T - \bar{\mu} \bar{x}_i^T - \bar{x}_i \bar{\mu}^T + \bar{\mu} \bar{\mu}^T)$$